theories/extraction.v
@@ -1,6 +1,6 @@
 (** Extraction to OCaml. **)
 (* (C) M. Bodin, J. Pichon - see LICENSE.txt *)
-
+(*
 From Coq Require Extraction.
 
 From Wasm Require Import
@@ -26,3 +26,4 @@ Extraction "extract"
   PP
   DummyHost.
 
+ *)
