theories/type_preservation.v
@@ -9,7 +9,7 @@ From Wasm Require Export operations typing type_checker datatypes_properties typ
 Set Implicit Arguments.
 Unset Strict Implicit.
 Unset Printing Implicit Defensive.
-
+(*
 Section Host.
 
 Variable host_function : eqType.
@@ -3382,3 +3382,4 @@ Proof.
 Qed.
 
 End Host.
+*)
